Use list based environment representation.
This eases proofs, because lists computes. It also avoids issues with duplicates (so, no
more environment splitting judgment, just append).

theories/logrel/environments.v
@@ -12,181 +12,188 @@ to the syntactic typing rules that are typically found in substructural type
 systems. *)
 From actris.logrel Require Export term_types subtyping.
 From iris.proofmode Require Import tactics.
+From iris.algebra Require Export list.
 
-Notation "<![ b := x ]!>" :=
-  (binder_insert b x%lty) (at level 5, right associativity).
+Inductive env_item Σ := EnvItem {
+  env_item_name : string;
+  env_item_type : ltty Σ;
+}.
+Add Printing Constructor env_item.
+Arguments EnvItem {_} _ _.
+Arguments env_item_name {_} _.
+Arguments env_item_type {_} _.
+Instance: Params (@EnvItem) 2 := {}.
+Instance: Params (@env_item_type) 1 := {}.
 
-Definition env_ltyped {Σ} (Γ : gmap string (ltty Σ))
-    (vs : gmap string val) : iProp Σ :=
-  ([∗ map] i ↦ A ∈ Γ, ∃ v, ⌜vs !! i = Some v⌝ ∗ ltty_car A v)%I.
+Section env_item_ofe.
+  Context {Σ : gFunctors}.
+  Instance env_item_equiv : Equiv (env_item Σ) := λ xA1 xA2,
+    env_item_name xA1 = env_item_name xA2 ∧ env_item_type xA1 ≡ env_item_type xA2.
+  Instance env_item_dist : Dist (env_item Σ) := λ n xA1 xA2,
+    env_item_name xA1 = env_item_name xA2 ∧ env_item_type xA1 ≡{n}≡ env_item_type xA2.
+  Lemma env_item_ofe_mixin : OfeMixin (env_item Σ).
+  Proof.
+    by apply (iso_ofe_mixin (A:=prodO (leibnizO string) (lttyO Σ))
+      (λ xA, (env_item_name xA, env_item_type xA))).
+  Qed.
+  Canonical Structure env_itemO := OfeT (env_item Σ) env_item_ofe_mixin.
+  Global Instance env_item_type_ne : NonExpansive (@env_item_type Σ).
+  Proof. by intros n ?? [??]. Qed.
+  Global Instance env_item_type_proper : Proper ((≡) ==> (≡)) (@env_item_type Σ).
+  Proof. by intros ?? [??]. Qed.
+End env_item_ofe.
 
-Definition env_split {Σ} (Γ Γ1 Γ2 : gmap string (ltty Σ)) : iProp Σ :=
-  (■ ∀ vs, env_ltyped Γ vs ∗-∗ (env_ltyped Γ1 vs ∗ env_ltyped Γ2 vs))%I.
+Notation env Σ := (list (env_item Σ)).
 
-Definition env_copy {Σ} (Γ Γ' : gmap string (ltty Σ)) : iProp Σ :=
-  (■ ∀ vs, env_ltyped Γ vs -∗ □ env_ltyped Γ' vs)%I.
+Definition env_filter_eq {Σ} (x : binder) : env Σ → env Σ :=
+  filter (λ xA, x = BNamed (env_item_name xA)).
+Definition env_filter_ne {Σ} (x : binder) : env Σ → env Σ :=
+  filter (λ xA, x ≠ BNamed (env_item_name xA)).
+
+Arguments env_filter_eq _ !_ !_ / : simpl nomatch.
+Arguments env_filter_ne _ !_ !_ / : simpl nomatch.
+(** TODO: Move to std++, together with some lemmas about filter that can be
+factored out. *)
+Arguments filter _ _ _ _ _ !_ / : simpl nomatch.
+
+Definition env_cons {Σ} (b : binder) (A : ltty Σ) (Γ : env Σ) : env Σ :=
+  if b is BNamed x then EnvItem x A :: env_filter_ne x Γ else Γ.
+
+Definition env_ltyped {Σ} (vs : gmap string val) (Γ : env Σ) : iProp Σ :=
+  ([∗ list] iA ∈ Γ, ∃ v,
+    ⌜vs !! env_item_name iA = Some v⌝ ∗ ltty_car (env_item_type iA) v)%I.
+Instance: Params (@env_ltyped) 2 := {}.
+
+Definition env_le {Σ} (Γ1 Γ2 : env Σ) : iProp Σ :=
+  tc_opaque (■ ∀ vs, env_ltyped vs Γ1 -∗ env_ltyped vs Γ2)%I.
+Instance: Params (@env_le) 1 := {}.
 
 Section env.
   Context {Σ : gFunctors}.
   Implicit Types A : ltty Σ.
-  Implicit Types Γ : gmap string (ltty Σ).
+  Implicit Types Γ : env Σ.
 
-  Lemma env_ltyped_empty vs : ⊢@{iPropI Σ} env_ltyped ∅ vs.
-  Proof. by iApply big_sepM_empty. Qed.
-
-  Lemma env_ltyped_lookup Γ vs x A :
-    Γ !! x = Some A →
-    env_ltyped Γ vs -∗
-    ∃ v, ⌜ vs !! x = Some v ⌝ ∗ ltty_car A v ∗ env_ltyped (delete x Γ) vs.
+  (** env_filter *)
+  Lemma env_filter_eq_perm Γ x : Γ ≡ₚ env_filter_eq x Γ ++ env_filter_ne x Γ.
   Proof.
-    iIntros (HΓx) "HΓ".
-    iPoseProof (big_sepM_delete with "HΓ") as "[HA H]"; eauto.
-    iDestruct "HA" as (v) "HA"; eauto with iFrame.
+    rewrite /env_filter_eq /env_filter_ne.
+    induction Γ as [|[y A] Γ IH]; simpl; [done|].
+    rewrite filter_cons. case_decide.
+    - rewrite filter_cons_False /=; last naive_solver. by rewrite -IH.
+    - rewrite filter_cons_True /=; last naive_solver.
+      by rewrite -Permutation_middle -IH.
+  Qed.
+  Lemma env_filter_eq_perm' Γ Γ' x :
+    env_filter_eq x Γ = Γ' →
+    Γ ≡ₚ Γ' ++ env_filter_ne x Γ.
+  Proof. intros <-. apply env_filter_eq_perm. Qed.
+
+  Lemma env_filter_ne_anon Γ : env_filter_ne BAnon Γ = Γ.
+  Proof. induction Γ as [|[y A] Γ IH]; by f_equal/=. Qed.
+
+  Lemma elem_of_env_filter_ne Γ x y B :
+    EnvItem y B ∈ env_filter_ne x Γ → x ≠ y.
+  Proof. intros ?%elem_of_list_filter. naive_solver. Qed.
+
+  Lemma env_filter_ne_cons Γ (x : string) A :
+    env_filter_ne x (EnvItem x A :: Γ) = env_filter_ne x Γ.
+  Proof. rewrite /env_filter_ne filter_cons_False; naive_solver. Qed.
+  Lemma env_filter_ne_cons_ne Γ x y A :
+    x ≠ BNamed y →
+    env_filter_ne x (EnvItem y A :: Γ) = EnvItem y A :: env_filter_ne x Γ.
+  Proof. intros. rewrite /env_filter_ne filter_cons_True; naive_solver. Qed.
+
+  (** env typing *)
+  Global Instance env_ltyped_Permutation vs :
+    Proper ((≡ₚ) ==> (⊣⊢)) (@env_ltyped Σ vs).	
+  Proof. intros Γ Γ' HΓ. by rewrite /env_ltyped HΓ. Qed.
+  Global Instance env_ltyped_ne vs : NonExpansive (@env_ltyped Σ vs).
+  Proof.
+    intros n Γ Γ' HΓ. rewrite /env_ltyped.
+    apply big_opL_gen_proper_2; [done|apply _|]. intros k.
+    assert (Γ !! k ≡{n}≡ Γ' !! k) as HΓk by (by rewrite HΓ).
+    case: HΓk=> // -[x1 A1] [x2 A2] [/= -> ?]. by repeat f_equiv.
+  Qed.
+  Global Instance env_ltyped_proper vs : Proper ((≡) ==> (≡)) (@env_ltyped Σ vs).
+  Proof. apply (ne_proper _). Qed.
+
+  Lemma env_ltyped_nil vs : ⊢@{iPropI Σ} env_ltyped vs [].
+  Proof. done. Qed.
+
+  Lemma env_ltyped_app Γ1 Γ2 vs :
+    env_ltyped vs (Γ1 ++ Γ2) ⊣⊢ env_ltyped vs Γ1 ∗ env_ltyped vs Γ2.
+  Proof. apply big_opL_app. Qed.
+
+  Lemma env_ltyped_cons Γ vs x A : 
+    env_ltyped vs (EnvItem x A :: Γ) ⊣⊢ ∃ v,
+    ⌜vs !! x = Some v⌝ ∗ ltty_car A v ∗ env_ltyped vs Γ.
+  Proof.
+    iSplit; [by iIntros "[HA $]"|].
+    iDestruct 1 as (v ?) "[HA $]"; eauto.
   Qed.
 
   Lemma env_ltyped_insert Γ vs x A v :
     ltty_car A v -∗
-    env_ltyped Γ vs -∗
-    env_ltyped (<![x:=A]!> Γ) (<![x:=v]!> vs).
+    env_ltyped vs (env_filter_ne x Γ) -∗
+    env_ltyped (binder_insert x v vs) (env_cons x A Γ).
   Proof.
-    destruct x as [|x]=> /=; first by auto.
     iIntros "HA HΓ".
-    rewrite /env_ltyped.
-    set Γ' := <[x:=A]> Γ.
-    assert (Hx: Γ' !! x = Some A).
-    { apply lookup_insert. }
-    iApply (big_sepM_delete _ _ _ _ Hx).
-    iSplitL "HA".
-    { iExists v. rewrite lookup_insert. auto. }
-    assert (Hsub: delete x Γ' ⊆ Γ).
-    { rewrite delete_insert_delete. apply delete_subseteq. }
-    iPoseProof (big_sepM_subseteq _ _ _ Hsub with "HΓ") as "HΓ".
-    iApply (big_sepM_mono with "HΓ"). simpl.
-    iIntros (y B Hy) "HB".
-    iDestruct "HB" as (w Hw) "HB".
-    iExists w. iFrame. iPureIntro.
-    apply lookup_delete_Some in Hy.
-    destruct Hy as [Hxy _].
-    by rewrite -Hw lookup_insert_ne.
+    destruct x as [|x]; simpl; [rewrite env_filter_ne_anon; auto|].
+    iApply env_ltyped_cons. iExists _; iSplit; [by rewrite lookup_insert|].
+    iFrame "HA". iApply (big_sepL_impl with "HΓ").
+    iIntros "!>" (k [j B] ?%elem_of_list_lookup_2%elem_of_env_filter_ne).
+    iDestruct 1 as (w ?) "HB". iExists w. iIntros "{$HB} !%".
+    apply lookup_insert_Some; naive_solver.
   Qed.
 
   Lemma env_ltyped_delete Γ x v vs :
-    env_ltyped Γ (<[x:=v]> vs) -∗
-    env_ltyped (delete x Γ) vs.
+    env_ltyped (binder_insert x v vs) Γ -∗
+    env_ltyped vs (env_filter_ne x Γ).
   Proof.
-    iIntros "HΓ".
-    rewrite /env_ltyped. destruct (Γ !! x) as [A|] eqn:?.
-    { iDestruct (big_sepM_delete with "HΓ") as "[HA HΓ]"; first done.
-      iDestruct "HA" as (v' ?) "HA"; simplify_map_eq.
-      iApply (big_sepM_impl with "HΓ").
-      iIntros "!>" (y B ?). iDestruct 1 as (v'' ?) "HB".
-      destruct (decide (x = y)); simplify_map_eq; eauto. }
-    rewrite delete_notin //. iApply (big_sepM_impl with "HΓ").
-    iIntros "!>" (y B ?). iDestruct 1 as (v' ?) "HB"; simplify_map_eq; eauto.
+    rewrite {1}(env_filter_eq_perm Γ x) env_ltyped_app. iIntros "[_ HΓ]".
+    iApply (big_sepL_impl with "HΓ").
+    iIntros "!>" (k [j B] ?%elem_of_list_lookup_2%elem_of_env_filter_ne).
+    iDestruct 1 as (w Hx) "HB". simpl in *. iExists w. iIntros "{$HB} !%".
+    destruct x as [|x]; simplify_eq/=; auto.
+    revert Hx. rewrite lookup_insert_Some. naive_solver.
   Qed.
 
-  Lemma env_split_id_l Γ : ⊢ env_split Γ ∅ Γ.
-  Proof.
-    iIntros "!>" (vs).
-    iSplit; [iIntros "$" | iIntros "[_ $]"]; iApply env_ltyped_empty.
-  Qed.
-  Lemma env_split_id_r Γ : ⊢ env_split Γ Γ ∅.
-  Proof.
-    iIntros "!>" (vs).
-    iSplit; [iIntros "$" | iIntros "[$ _]"]; iApply env_ltyped_empty.
-  Qed.
+  (** Environment subtyping *)
+  Global Instance env_le_plain Γ1 Γ2 : Plain (env_le Γ1 Γ2).
+  Proof. rewrite /env_le /=. apply _. Qed.
 
-  Lemma env_split_empty : ⊢@{iPropI Σ} env_split ∅ ∅ ∅.
+  Global Instance env_le_Permutation : Proper ((≡ₚ) ==> (≡ₚ) ==> (≡)) (@env_le Σ).
   Proof.
-    iIntros "!>" (vs).
-    iSplit; [iIntros "HΓ" | iIntros "[HΓ1 HΓ2]"]; auto.
+    intros Γ1 Γ1' HΓ1 Γ2 Γ2' HΓ2. rewrite /env_le /=.
+    setoid_rewrite HΓ1; by setoid_rewrite HΓ2.
   Qed.
+  Global Instance env_le_ne : NonExpansive2 (@env_le Σ).
+  Proof. solve_proper. Qed.
+  Global Instance env_le_proper : Proper ((≡) ==> (≡) ==> (≡)) (@env_le Σ).
+  Proof. apply (ne_proper_2 _). Qed.
 
-  (* TODO: Get rid of side condition that x does not appear in Γ1 *)
-  Lemma env_split_left Γ Γ1 Γ2 x A:
-    Γ !! x = None → Γ1 !! x = None →
-    env_split Γ Γ1 Γ2 -∗
-    env_split (<[x := A]> Γ) (<[x := A]> Γ1) Γ2.
+  Lemma env_le_refl Γ : ⊢ env_le Γ Γ.
+  Proof. iIntros (vs); auto. Qed.
+  Lemma env_le_trans Γ1 Γ2 Γ3 : env_le Γ1 Γ2 -∗ env_le Γ2 Γ3 -∗ env_le Γ1 Γ3.
   Proof.
-    iIntros (HΓx HΓ2x) "#Hsplit !>". iIntros (vs).
-    iSplit.
-    - iIntros "HΓ".
-      iPoseProof (big_sepM_insert with "HΓ") as "[Hv HΓ]"; first by assumption.
-      iDestruct ("Hsplit" with "HΓ") as "[HΓ1 $]".
-      iApply (big_sepM_insert_2 with "[Hv]"); simpl; eauto.
-    - iIntros "[HΓ1 HΓ2]".
-      iPoseProof (big_sepM_insert with "HΓ1") as "[Hv HΓ1]"; first by assumption.
-      iApply (big_sepM_insert_2 with "[Hv]")=> //.
-      iApply "Hsplit". iFrame "HΓ1 HΓ2".
+    rewrite /env_le /=.
+    iIntros "#H1 #H2 !>" (vs) "Hvs". iApply "H2". by iApply "H1".
   Qed.
-
-  Lemma env_split_comm Γ Γ1 Γ2:
-    env_split Γ Γ1 Γ2 -∗ env_split Γ Γ2 Γ1.
+  Lemma env_le_nil Γ : ⊢ env_le Γ [].
+  Proof. iIntros (vs) "!> _". iApply env_ltyped_nil. Qed.
+  Lemma env_le_cons x Γ1 Γ2 A1 A2 :
+    A1 <: A2 -∗ env_le Γ1 Γ2 -∗ env_le (EnvItem x A1 :: Γ1) (EnvItem x A2 :: Γ2).
   Proof.
-    iIntros "#Hsplit" (vs) "!>".
-    iSplit.
-    - iIntros "HΓ". by iDestruct ("Hsplit" with "HΓ") as "[$ $]".
-    - iIntros "[HΓ1 HΓ2]". iApply "Hsplit". iFrame.
+    rewrite /env_le /=. iIntros "#H #H' !>" (vs) "Hvs".
+    iDestruct (env_ltyped_cons with "Hvs") as (v ?) "[Hv Hvs]".
+    iApply env_ltyped_cons. iExists _; iSplit; [done|].
+    iSplitL "Hv"; [by iApply "H"|by iApply "H'"].
   Qed.
-
-  (* TODO: Get rid of side condition that x does not appear in Γ2 *)
-  Lemma env_split_right Γ Γ1 Γ2 x A:
-    Γ !! x = None → Γ2 !! x = None →
-    env_split Γ Γ1 Γ2 -∗
-    env_split (<[x := A]> Γ) Γ1 (<[x := A]> Γ2).
+  Lemma env_le_app Γ1 Γ2 Γ1' Γ2' :
+    env_le Γ1 Γ2 -∗ env_le Γ1' Γ2' -∗ env_le (Γ1 ++ Γ1') (Γ2 ++ Γ2').
   Proof.
-    iIntros (HΓx HΓ2x) "Hsplit".
-    iApply env_split_comm. iApply env_split_left=> //.
-    by iApply env_split_comm.
-  Qed.
-
-  (* TODO: Get rid of side condition that x does not appear in Γ *)
-  Lemma env_split_copyable Γ Γ1 Γ2 (x : string) A:
-    Γ !! x = None → Γ1 !! x = None → Γ2 !! x = None →
-    lty_copyable A -∗
-    env_split Γ Γ1 Γ2 -∗
-    env_split (<[x:=A]> Γ) (<[x:=A]> Γ1) (<[x:=A]> Γ2).
-  Proof.
-    iIntros (HΓx HΓ1x HΓ2x) "#Hcopy #Hsplit". iIntros (vs) "!>".
-    iSplit.
-    - iIntros "HΓ".
-      iPoseProof (big_sepM_insert with "HΓ") as "[Hv HΓ]"; first by assumption.
-      iDestruct "Hv" as (v ?) "HAv2".
-      iDestruct ("Hcopy" with "HAv2") as "#HAv".
-      iDestruct ("Hsplit" with "HΓ") as "[HΓ1 HΓ2]".
-      iSplitL "HΓ1"; iApply big_sepM_insert_2; simpl; eauto.
-    - iIntros "[HΓ1 HΓ2]".
-      iPoseProof (big_sepM_insert with "HΓ1") as "[Hv HΓ1]"; first by assumption.
-      iPoseProof (big_sepM_insert with "HΓ2") as "[_ HΓ2]"; first by assumption.
-      iApply (big_sepM_insert_2 with "[Hv]")=> //.
-      iApply "Hsplit". iFrame "HΓ1 HΓ2".
-  Qed.
-
-  Lemma env_copy_empty : ⊢@{iPropI Σ} env_copy ∅ ∅.
-  Proof. iIntros (vs) "!> _ !> ". by rewrite /env_ltyped. Qed.
-
-  Lemma env_copy_extend x A Γ Γ' :
-    Γ !! x = None →
-    env_copy Γ Γ' -∗
-    env_copy (<[x:=A]> Γ) Γ'.
-  Proof.
-    iIntros (HΓ) "#Hcopy". iIntros (vs) "!> Hvs". rewrite /env_ltyped.
-    iDestruct (big_sepM_insert with "Hvs") as "[_ Hvs]"; first by assumption.
-    iApply ("Hcopy" with "Hvs").
-  Qed.
-
-  Lemma env_copy_extend_copyable x A Γ Γ' :
-    Γ !! x = None →
-    Γ' !! x = None →
-    lty_copyable A -∗
-    env_copy Γ Γ' -∗
-    env_copy (<[x:=A]> Γ) (<[x:=A]> Γ').
-  Proof.
-    iIntros (HΓx HΓ'x) "#HcopyA #Hcopy". iIntros (vs) "!> Hvs". rewrite /env_ltyped.
-    iDestruct (big_sepM_insert with "Hvs") as "[HA Hvs]"; first done.
-    iDestruct ("Hcopy" with "Hvs") as "#Hvs'".
-    iDestruct "HA" as (v ?) "HA2".
-    iDestruct ("HcopyA" with "HA2") as "#HA".
-    iIntros "!>". iApply big_sepM_insert; first done. iSplitL; eauto.
+    rewrite /env_le /=. iIntros "#H #H' !>" (vs) "Hvs".
+    iDestruct (env_ltyped_app with "Hvs") as "[Hvs1 Hvs2]".
+    iApply env_ltyped_app. iSplitL "Hvs1"; [by iApply "H"|by iApply "H'"].
   Qed.
 End env.
