theories/logrel/lib/mutex.v
@@ -40,12 +40,12 @@ Definition mutex_release : val :=
 (** Semantic types *)
 Definition lty_mutex `{heapG Σ, lockG Σ} (A : ltty Σ) : ltty Σ := Ltty (λ w,
   ∃ (γ : gname) (l : loc) (lk : val),
-    ⌜ w = PairV lk #l ⌝ ∗
+    ⌜ w = (lk,#l)%V ⌝ ∗
     is_lock γ lk (∃ v_inner, l ↦ v_inner ∗ ltty_car A v_inner))%I.
 
 Definition lty_mutex_guard `{heapG Σ, lockG Σ} (A : ltty Σ) : ltty Σ := Ltty (λ w,
   ∃ (γ : gname) (l : loc) (lk : val) (v : val),
-    ⌜ w = PairV lk #l ⌝ ∗
+    ⌜ w = (lk,#l)%V ⌝ ∗
     is_lock γ lk (∃ v_inner, l ↦ v_inner ∗ ltty_car A v_inner) ∗
     spin_lock.locked γ ∗ l ↦ v)%I.
 
@@ -64,8 +64,7 @@ Section properties.
   Global Instance lty_mutex_ne : NonExpansive lty_mutex.
   Proof. solve_proper. Qed.
 
-  Global Instance lty_mutex_guard_contractive :
-    Contractive lty_mutex_guard.
+  Global Instance lty_mutex_guard_contractive : Contractive lty_mutex_guard.
   Proof. solve_contractive. Qed.
   Global Instance lty_mutex_guard_ne : NonExpansive lty_mutex_guard.
   Proof. solve_proper. Qed.
@@ -108,64 +107,47 @@ Section rules.
     ⊢ Γ ⊨ mutex_alloc : A → mutex A ⫤ Γ.
   Proof.
     iIntros (vs) "!> HΓ /=". iApply wp_value.
-    iFrame "HΓ".
-    iIntros "!>" (v) "Hv". rewrite /mutex_alloc. wp_pures.
+    iIntros "{$HΓ} !>" (v) "Hv". rewrite /mutex_alloc. wp_pures.
     wp_alloc l as "Hl".
-    wp_bind (newlock _).
     set (N := nroot .@ "makelock").
     iAssert (∃ inner, l ↦ inner ∗ ltty_car A inner)%I with "[Hl Hv]" as "Hlock".
     { iExists v. iFrame "Hl Hv". }
     wp_apply (newlock_spec with "Hlock").
     iIntros (lk γ) "Hlock".
-    wp_pures. iExists γ, l, lk. iSplit=> //.
+    wp_pures. iExists γ, l, lk. eauto.
   Qed.
 
   Lemma ltyped_mutex_acquire Γ (x : string) A :
-    Γ !! x = Some (mutex A)%lty →
-    ⊢ Γ ⊨ mutex_acquire x : A ⫤ <[x := (mutex_guard A)%lty]> Γ.
+    env_filter_eq x Γ = [EnvItem x (mutex A)] →
+    ⊢ Γ ⊨ mutex_acquire x : A ⫤ env_cons x (mutex_guard A) Γ.
   Proof.
-    iIntros (Hx vs) "!> HΓ /=".
-    iDestruct (env_ltyped_lookup with "HΓ") as (v Hv) "[HA HΓ]"; first done; rewrite Hv.
-    rewrite /mutex_acquire. wp_pures.
-    iDestruct "HA" as (γ l lk ->) "#Hlock".
-    wp_bind (acquire _).
-    wp_apply (acquire_spec with "Hlock"). iIntros "[Hlocked Hinner]".
+    iIntros (HΓx%env_filter_eq_perm' vs) "!> HΓ /=". rewrite {1}HΓx /=.
+    iDestruct (env_ltyped_cons with "HΓ") as (vl Hvs) "[Hlock HΓ]"; rewrite Hvs.
+    iDestruct "Hlock" as (γ l lk ->) "#Hlock". rewrite /mutex_acquire.
+    wp_apply (acquire_spec with "Hlock"); iIntros "[Hlocked Hinner]".
     iDestruct "Hinner" as (v) "[Hl HA]".
-    wp_pures. wp_load.
-    iFrame "HA".
-    iAssert (ltty_car (mutex_guard A)%lty (lk, #l)) with "[Hlocked Hl]" as "Hguard".
-    { iExists γ, l, lk, v. iSplit=>//. iFrame "Hlocked Hl Hlock". }
-    iDestruct (env_ltyped_insert _ _ x with "Hguard HΓ") as "HΓ".
-    rewrite /binder_insert insert_delete (insert_id _ _ _ Hv).
-    iFrame "HΓ".
+    wp_load. iFrame "HA". iApply env_ltyped_cons.
+    iFrame "HΓ". iExists _; iSplit; [done|]. iExists γ, l, lk, v. auto with iFrame.
   Qed.
 
   Lemma ltyped_mutex_release Γ Γ' (x : string) e A :
-    Γ' !! x = Some (mutex_guard A)%lty →
+    env_filter_eq x Γ' = [EnvItem x (mutex_guard A)] →
     (Γ ⊨ e : A ⫤ Γ') -∗
-    Γ ⊨ mutex_release x e : () ⫤ <[x := (mutex A)%lty]> Γ'.
+    Γ ⊨ mutex_release x e : () ⫤ env_cons x (mutex A) Γ'.
   Proof.
-    iIntros (Hx) "#He". iIntros (vs) "!> HΓ /=".
-    wp_bind (subst_map vs e).
-    iApply (wp_wand with "(He HΓ)"). iIntros (v) "[HA HΓ']".
-    iDestruct (env_ltyped_lookup with "HΓ'") as (g Hg) "[Hguard HΓ']"; first done; rewrite Hg.
+    iIntros (HΓx%env_filter_eq_perm') "#He". iIntros (vs) "!> HΓ /=".
+    wp_apply (wp_wand with "(He HΓ)"). iIntros (v) "[HA HΓ']".
+    rewrite {2}HΓx /=.
+    iDestruct (env_ltyped_cons with "HΓ'") as (vl Hvs) "[Hguard HΓ']"; rewrite Hvs.
     iDestruct "Hguard" as (γ l lk inner ->) "(#Hlock & Hlocked & Hinner)".
-    rewrite /mutex_release.
-    wp_pures. wp_store. wp_pures.
+    rewrite /mutex_release. wp_store.
     iAssert (∃ inner, l ↦ inner ∗ ltty_car A inner)%I
       with "[Hinner HA]" as "Hinner".
     { iExists v. iFrame "Hinner HA". }
     wp_apply (release_spec γ _ (∃ inner, l ↦ inner ∗ ltty_car A inner)%I
-                with "[Hlocked Hinner]").
-    { iFrame "Hlock Hlocked".
-      iDestruct "Hinner" as (w) "[Hl HA]". eauto with iFrame. }
-    iIntros "_". wp_pures.
-    iSplit=> //.
-    iAssert (ltty_car (mutex A)%lty (lk, #l)) with "[Hlock]" as "Hmutex".
-    { iExists γ, l, lk. iSplit=>//. }
-    iDestruct (env_ltyped_insert _ _ x with "Hmutex HΓ'") as "HΓ'".
-    rewrite /binder_insert insert_delete (insert_id _ _ _ Hg).
-    iFrame "HΓ'".
+      with "[$Hlock $Hlocked $Hinner]").
+    iIntros "_". iSplit; [done|].
+    iApply env_ltyped_cons. iFrame "HΓ'". iExists _; iSplit; [done|].
+    iExists γ, l, lk. auto.
   Qed.
-
 End rules.
