theories/logrel/term_typing_judgment.v
@@ -8,27 +8,47 @@ programs which satisfy the semantic typing relation are safe. That is,
 semantically well-typed programs do not get stuck. *)
 From iris.heap_lang Require Import metatheory adequacy.
 From actris.logrel Require Export term_types.
-From actris.logrel Require Import environments.
+From actris.logrel Require Export environments.
 From iris.proofmode Require Import tactics.
 
 (** The semantic typing judgment *)
 Definition ltyped `{!heapG Σ}
-    (Γ Γ' : gmap string (ltty Σ)) (e : expr) (A : ltty Σ) : iProp Σ :=
-  (■ ∀ vs, env_ltyped Γ vs -∗
-           WP subst_map vs e {{ v, ltty_car A v ∗ env_ltyped Γ' vs }})%I.
+    (Γ1 Γ2 : env Σ) (e : expr) (A : ltty Σ) : iProp Σ :=
+  tc_opaque (■ ∀ vs, env_ltyped vs Γ1 -∗
+    WP subst_map vs e {{ v, ltty_car A v ∗ env_ltyped vs Γ2 }})%I.
+Instance: Params (@ltyped) 2 := {}.
 
-Notation "Γ ⊨ e : A ⫤ Γ'" := (ltyped Γ Γ' e A)
+Notation "Γ1 ⊨ e : A ⫤ Γ2" := (ltyped Γ1 Γ2 e A)
   (at level 100, e at next level, A at level 200).
 Notation "Γ ⊨ e : A" := (Γ ⊨ e : A ⫤ Γ)
   (at level 100, e at next level, A at level 200).
 
+Section ltyped.
+  Context `{!heapG Σ}.
+
+  Global Instance ltyped_plain Γ1 Γ2 e A : Plain (ltyped Γ1 Γ2 e A).
+  Proof. rewrite /ltyped /=. apply _. Qed.
+  Global Instance ltyped_ne n :
+    Proper (dist n ==> dist n ==> (=) ==> dist n ==> dist n) (@ltyped Σ _).
+  Proof. solve_proper. Qed.
+  Global Instance ltyped_proper :
+    Proper ((≡) ==> (≡) ==> (=) ==> (≡) ==> (≡)) (@ltyped Σ _).
+  Proof. solve_proper. Qed.
+  Global Instance ltyped_Permutation :
+    Proper ((≡ₚ) ==> (≡ₚ) ==> (=) ==> (≡) ==> (≡)) (@ltyped Σ _).
+  Proof.
+    intros Γ1 Γ1' HΓ1 Γ2 Γ2' HΓ2 e ? <- A ? <-. rewrite /ltyped /=.
+    setoid_rewrite HΓ1. by setoid_rewrite HΓ2.
+  Qed.
+End ltyped.
+
 Lemma ltyped_safety `{heapPreG Σ} e σ es σ' e' :
-  (∀ `{heapG Σ}, ∃ A Γ', ⊢ ∅ ⊨ e : A ⫤ Γ') →
+  (∀ `{heapG Σ}, ∃ A, ⊢ [] ⊨ e : A ⫤ []) →
   rtc erased_step ([e], σ) (es, σ') → e' ∈ es →
   is_Some (to_val e') ∨ reducible e' σ'.
 Proof.
   intros Hty. apply (heap_adequacy Σ NotStuck e σ (λ _, True))=> // ?.
-  destruct (Hty _) as (A & Γ' & He). iIntros "_".
+  destruct (Hty _) as (A & He). iIntros "_".
   iDestruct (He $!∅ with "[]") as "He"; first by rewrite /env_ltyped.
   iEval (rewrite -(subst_map_empty e)). iApply (wp_wand with "He"); auto.
 Qed.
